- Add more premises in proving that precondition and postcondition   are safe. - Add fe25519_sub in bvDSL.

mqhasm/bvDSL2zDSL.v
@@ -457,9 +457,10 @@ Definition bv2z_spec_poly s : zDSL.spec :=
      zDSL.spost := bv2z_ebexp (fst (split_bexp (spost s))) |}.
 
 Definition bv2z_spec_safe sp :=
-  (forall s, eval_bexp (spre sp) s -> bv2z_program_safe_at (sprog sp) s) /\
   (forall s, bv2z_bexp_safe_at (spre sp) s) /\
-  (forall s, bv2z_bexp_safe_at (spost sp) s).
+  (forall s, eval_bexp (spre sp) s -> bv2z_program_safe_at (sprog sp) s) /\
+  (forall s s', eval_bexp (spre sp) s -> eval_program s (sprog sp) = s' ->
+                bv2z_bexp_safe_at (spost sp) s').
 
 
 
@@ -870,14 +871,14 @@ Lemma bv2z_spec_sound sp :
   valid_spec sp.
 Proof.
   destruct sp as [f p g] => /=.
-  move=> [/= Hsafep [Hsafef Hsafeg]] Hrng Heqn bs1 bs2 /= Hbf Hbp.
+  move=> [/= Hsafef [Hsafep Hsafeg]] Hrng Heqn bs1 bs2 /= Hbf Hbp.
   move: (Hrng bs1 bs2 Hbf Hbp) => {Hrng} /= Hrng.
   set zs1 := bv2z_state bs1.
   set zs2 := zDSL.eval_program zs1 (bv2z_program p).
   move: (Heqn zs1 zs2
               (bvz_eq_eval_bexp (Hsafef bs1) (bv2z_state_eq bs1) Hbf)
               (Logic.eq_refl zs2)) => {Heqn} /= Heqn.
-  apply: (@split_bexp_combine g bs2 zs2 (Hsafeg bs2) _ Hrng Heqn).
+  apply: (@split_bexp_combine g bs2 zs2 (Hsafeg bs1 bs2 Hbf Hbp) _ Hrng Heqn).
   rewrite -Hbp.
   exact: (bvz_eq_eval_program (bv2z_state_eq bs1) (Hsafep _ Hbf)).
 Qed.
