fe25519/bvdsl/fe25519_sub.v
@@ -1,0 +1,185 @@
+
+From Coq Require Import ZArith.
+From mathcomp Require Import ssreflect ssrbool ssrnat seq.
+From Common Require Import Bits.
+From mQhasm Require Import bvDSL bvVerify Options.
+
+Set Implicit Arguments.
+Unset Strict Implicit.
+Import Prenex Implicits.
+
+
+
+Open Scope N_scope.
+Open Scope bvdsl_scope.
+
+Definition fe25519_sub : program :=
+
+let crypto_sign_ed25519_amd64_51_2P0 :=
+                       4503599627370458%Z in (* 0xFFFFFFFFFFFDA from consts *)
+let crypto_sign_ed25519_amd64_51_2P1234 :=
+                       4503599627370494%Z in (* 0xFFFFFFFFFFFFE from consts *)
+
+let            x0 :=   0 in
+let            x1 :=   1 in
+let            x2 :=   2 in
+let            x3 :=   3 in
+let            x4 :=   4 in
+
+let            y0 :=   5 in
+let            y1 :=   6 in
+let            y2 :=   7 in
+let            y3 :=   8 in
+let            y4 :=   9 in
+
+let            r0 :=  20 in
+let            r1 :=  21 in
+let            r2 :=  22 in
+let            r3 :=  23 in
+let            r4 :=  24 in
+[::
+      (* # CPU: Intel(R) Xeon(R) CPU X5675 @ 3.07GHz *)
+      (* # RAM: 32GB *)
+      (* # Configuration: -c consts -s *)
+      (* # With Boolector 1.6.0 (-minisat): 3m38.621s *)
+      (*  *)
+      (* int64 x0 *)
+      (* int64 x1 *)
+      (* int64 x2 *)
+      (* int64 x3 *)
+      (* int64 x4 *)
+      (*  *)
+      (* int64 y0 *)
+      (* int64 y1 *)
+      (* int64 y2 *)
+      (* int64 y3 *)
+      (* int64 y4 *)
+      (*  *)
+      (* int64 r0 *)
+      (* int64 r1 *)
+      (* int64 r2 *)
+      (* int64 r3 *)
+      (* int64 r4 *)
+      (*  *)
+      (* #// assume 0 <=u x0, x1, x2, x3, x4, y0, y1, y2, y3, y4 <=u 2**51 + 2**15 *)
+      (*  *)
+      (* r0 = x0 *)
+bvAssign r0 (bvVar x0);
+      (* r1 = x1 *)
+bvAssign r1 (bvVar x1);
+      (* r2 = x2 *)
+bvAssign r2 (bvVar x2);
+      (* r3 = x3 *)
+bvAssign r3 (bvVar x3);
+      (* r4 = x4 *)
+bvAssign r4 (bvVar x4);
+      (* r0 += *[uint64 *] &crypto_sign_ed25519_amd64_51_2P0 *)
+bvAdd r0 (bvVar r0) (bvConst (fromPosZ crypto_sign_ed25519_amd64_51_2P0));
+      (* r1 += *[uint64 *] &crypto_sign_ed25519_amd64_51_2P1234 *)
+bvAdd r1 (bvVar r1) (bvConst (fromPosZ crypto_sign_ed25519_amd64_51_2P1234));
+      (* r2 += *[uint64 *] &crypto_sign_ed25519_amd64_51_2P1234 *)
+bvAdd r2 (bvVar r2) (bvConst (fromPosZ crypto_sign_ed25519_amd64_51_2P1234));
+      (* r3 += *[uint64 *] &crypto_sign_ed25519_amd64_51_2P1234 *)
+bvAdd r3 (bvVar r3) (bvConst (fromPosZ crypto_sign_ed25519_amd64_51_2P1234));
+      (* r4 += *[uint64 *] &crypto_sign_ed25519_amd64_51_2P1234 *)
+bvAdd r4 (bvVar r4) (bvConst (fromPosZ crypto_sign_ed25519_amd64_51_2P1234));
+      (* r0 -= y0 *)
+bvSub r0 (bvVar r0) (bvVar y0);
+      (* r1 -= y1 *)
+bvSub r1 (bvVar r1) (bvVar y1);
+      (* r2 -= y2 *)
+bvSub r2 (bvVar r2) (bvVar y2);
+      (* r3 -= y3 *)
+bvSub r3 (bvVar r3) (bvVar y3);
+      (* r4 -= y4 *)
+bvSub r4 (bvVar r4) (bvVar y4)
+      (*  *)
+      (* #// var sum_x = x0@u320 + x1@u320 * 2**51 + x2@u320 * 2**102 + x3@u320 * 2**153 + x4@u320 * 2**204 *)
+      (* #//     sum_y = y0@u320 + y1@u320 * 2**51 + y2@u320 * 2**102 + y3@u320 * 2**153 + y4@u320 * 2**204 *)
+      (* #//     sum_r = r0@u320 + r1@u320 * 2**51 + r2@u320 * 2**102 + r3@u320 * 2**153 + r4@u320 * 2**204 *)
+      (* #// assert (sum_r - (sum_x - sum_y)) % (2**255 - 19) = 0 && *)
+      (* #//        0 <=u r0, r1, r2, r3, r4 <u 2**54 *)
+] .
+
+Definition fe25519_sub_inputs : VS.t :=
+let            x0 :=   0 in
+let            x1 :=   1 in
+let            x2 :=   2 in
+let            x3 :=   3 in
+let            x4 :=   4 in
+let            y0 :=   5 in
+let            y1 :=   6 in
+let            y2 :=   7 in
+let            y3 :=   8 in
+let            y4 :=   9 in
+VSLemmas.OP.P.of_list [:: x0; x1; x2; x3; x4; y0; y1; y2; y3; y4].
+
+Definition fe25519_sub_pre : bexp :=
+let            x0 :=   0 in
+let            x1 :=   1 in
+let            x2 :=   2 in
+let            x3 :=   3 in
+let            x4 :=   4 in
+let            y0 :=   5 in
+let            y1 :=   6 in
+let            y2 :=   7 in
+let            y3 :=   8 in
+let            y4 :=   9 in
+bvands
+  [::
+     bvult (bvvar x0) (bvposz (2^51 + 2^15)%Z);
+     bvult (bvvar x1) (bvposz (2^51 + 2^15)%Z);
+     bvult (bvvar x2) (bvposz (2^51 + 2^15)%Z);
+     bvult (bvvar x3) (bvposz (2^51 + 2^15)%Z);
+     bvult (bvvar x4) (bvposz (2^51 + 2^15)%Z);
+     bvult (bvvar y0) (bvposz (2^51 + 2^15)%Z);
+     bvult (bvvar y1) (bvposz (2^51 + 2^15)%Z);
+     bvult (bvvar y2) (bvposz (2^51 + 2^15)%Z);
+     bvult (bvvar y3) (bvposz (2^51 + 2^15)%Z);
+     bvult (bvvar y4) (bvposz (2^51 + 2^15)%Z)
+  ].
+
+Definition radix51 := @limbs 51 320.
+
+Definition fe25519_sub_post : bexp :=
+let            x0 :=   0 in
+let            x1 :=   1 in
+let            x2 :=   2 in
+let            x3 :=   3 in
+let            x4 :=   4 in
+let            y0 :=   5 in
+let            y1 :=   6 in
+let            y2 :=   7 in
+let            y3 :=   8 in
+let            y4 :=   9 in
+let            r0 :=  20 in
+let            r1 :=  21 in
+let            r2 :=  22 in
+let            r3 :=  23 in
+let            r4 :=  24 in
+let        n25519 := 57896044618658097711785492504343953926634992332820282019728792003956564819949%Z in
+bvEqMod
+  (
+    (
+      (radix51 [:: bvvar x0; bvvar x1; bvvar x2; bvvar x3; bvvar x4])
+      @+
+      (bvposz n25519 @* bvposz 31%Z)
+    )
+    @-
+    (radix51 [:: bvvar y0; bvvar y1; bvvar y2; bvvar y3; bvvar y4])
+  )
+  (radix51 [:: bvvar r0; bvvar r1; bvvar r2; bvvar r3; bvvar r4])
+  (bvposz n25519).
+
+Definition fe25519_sub_spec :=
+  {| spre := fe25519_sub_pre;
+     sprog := fe25519_sub;
+     spost := fe25519_sub_post |}.
+
+Lemma valid_fe25519_sub : valid_bvspec (fe25519_sub_inputs, fe25519_sub_spec).
+Proof.
+  time "valid_fe25519_sub" verify_bvspec.
+Qed.
+
+Close Scope bvdsl_scope.
+Close Scope N_scope.
